LeanSubst.lean
@@ -1,6 +1,7 @@
--- This module serves as the root of the `LeanSubst` library.
--- Import modules here that should be built as part of the library.
+
 import LeanSubst.Basic
+import LeanSubst.Arity
+import LeanSubst.Context
 import LeanSubst.Map
 import LeanSubst.Reduction
 import LeanSubst.Normal
