LeanSubst/Context.lean
@@ -1,0 +1,35 @@
+import LeanSubst.Basic
+
+namespace LeanSubst
+
+variable {T : Type} [Inhabited T] [SubstMap T]
+
+inductive Ctx (T : Type) where
+| nil : Ctx T
+| cons : T -> Ctx T -> Ctx T
+
+notation "[]" => Ctx.nil
+infixr:55 "::" => Ctx.cons
+
+@[simp]
+def nth : Ctx T -> Nat -> T
+| [], _ => default
+| .cons h _, 0 => h
+| .cons _ t, n + 1 => nth t n
+
+@[simp]
+def Ctx.dnth : Ctx T -> Nat -> T
+| .nil, _ => default
+| .cons h _, 0 => h[+1]
+| .cons _ t, n + 1 => (dnth t n)[+1]
+
+instance : GetElem (Ctx T) Nat T (λ _ _ => True) where
+  getElem := λ Γ x _ => Ctx.dnth Γ x
+
+@[simp]
+theorem Ctx.elem_cons_zero {A : T} {Γ : Ctx T} : (A::Γ)[0] = A[+1] := by simp [getElem]
+
+@[simp]
+theorem Ctx.elem_cons_succ {A : T} {Γ : Ctx T} {x} : (A::Γ)[x + 1] = Γ[x][+1] := by simp [getElem]
+
+end LeanSubst
